Reorganisation + comments.

coq-osiris/theories/adequacy/ewp_adequacy.v
@@ -24,12 +24,9 @@ Definition is_join {A E} (m : micro A E) : Prop :=
 Definition not_stuck {A E} (m : micro A E) σ (π : gset thread) :=
   is_final m ∨ can_progress σ π m ∨ is_join m.
 
-Lemma wp_wptp `{!osirisGS Σ} ι m γ φ :
-  (saved_pred_own γ DfracDiscarded φ ∗ EWP m @ ⊤ <| (ι, ⊥) |> {{ λ o, □ φ o }}) ⊣⊢ WPTP {[ι := m ]} {[ι := (γ, φ)]}.
-Proof.
-  unfold WPTP.
-  by rewrite big_sepM2_singleton.
-Qed.
+
+(* -------------------------------------------------------------------------- *)
+(* General gmap helper lemmas *)
 
 Lemma not_elem_of_lookup {K} `{FinMapDom K M D} {A} (ι ι' : K) (π : M A) (m : A) :
   ι' ≠ ι ->
@@ -45,14 +42,70 @@ Proof.
   - apply not_elem_of_dom. apply Hlookup.
 Qed.
 
-Lemma wptp_dom `{!osirisGS Σ} m F Rs π πp :
-  SAT m F Rs (WPTP π πp) → dom πp ≡ dom π.
+Lemma fmap_fst_lookup {A B} (m : gmap thread (A * B)) ι a b :
+  m !! ι = Some (a, b) →
+  (fst <$> m) !! ι = Some a.
+Proof. intros. by rewrite lookup_fmap H. Qed.
+
+Lemma lookup_delete_ne_inv {K} `{Countable K} {A} (m : gmap K A) (i j : K) (x : A) :
+  i ≠ j →
+  m !! j = Some x →
+  delete i m !! j = Some x.
+Proof. intros. by rewrite lookup_delete_ne. Qed.
+
+(* [insert_list] takes a list of bindings, a gmap,
+   and inserts every binding into the gmap in order. *)
+Fixpoint insert_list {A : Type} l (πp : gmap thread A) :=
+    match l with
+    | [] => πp
+    | (ι, φ) :: t => <[ι:=φ]>(insert_list t πp)
+    end.
+
+Lemma insert_list_app {A : Type} l l' (πp : gmap thread A) :
+  insert_list (l' ++ l) πp = insert_list l' (insert_list l πp).
 Proof.
-  intros Hsat.
-  eapply SAT_elim, SAT_mono, Hsat.
-  iIntros "Hwps".
-  iPoseProof (big_sepM2_dom with "Hwps") as "%Hdomeq".
-  iPureIntro. by rewrite Hdomeq.
+  induction l' as [ | [ι' φ'] l'].
+  - reflexivity.
+  - simpl. f_equal.
+    apply IHl'.
+Qed.
+
+Lemma insert_list_lookup_not_in {A} ι l (πp : gmap thread A) :
+  ι ∉ fst <$> l →
+  insert_list l πp !! ι = πp !! ι.
+Proof.
+  induction l as [| [ι' a] l IH]; first done.
+  rewrite fmap_cons not_elem_of_cons. simpl.
+  intros [Hneq Hnin].
+  rewrite lookup_insert_ne; first by apply IH.
+  by symmetry.
+Qed.
+
+Lemma not_elem_of_insert_list {A} ι l (πp : gmap thread A) :
+  ι ∉ dom (insert_list l πp) →
+  ι ∉ fst <$> l ∧ ι ∉ dom πp.
+Proof.
+  induction l as [| [ι' a] l IH].
+  - simpl.
+    intros Hnin.
+    split; [ apply not_elem_of_nil | exact Hnin ].
+  - simpl. rewrite dom_insert.
+    rewrite not_elem_of_union not_elem_of_singleton.
+    intros [Hnhead Hndom].
+    destruct (IH Hndom) as [Hnlist Hndom'].
+    rewrite not_elem_of_cons.
+    auto.
+Qed.
+
+(* -------------------------------------------------------------------------- *)
+(* Helper lemmas for manipulating [WPTP]s. *)
+
+(* [wp_wptp] established the correspondence between [EWP] and [WPTP] over a singleton. *)
+Lemma wp_wptp `{!osirisGS Σ} ι m γ φ :
+  (saved_pred_own γ DfracDiscarded φ ∗ EWP m @ ⊤ <| (ι, ⊥) |> {{ λ o, □ φ o }}) ⊣⊢ WPTP {[ι := m ]} {[ι := (γ, φ)]}.
+Proof.
+  unfold WPTP.
+  by rewrite big_sepM2_singleton.
 Qed.
 
 Lemma WPTP_dom `{!osirisGS Σ} π πp :
@@ -63,6 +116,15 @@ Proof.
   by iPureIntro.
 Qed.
 
+Lemma WPTP_dom_equiv `{!osirisGS Σ} π πp :
+  WPTP π πp -∗ ⌜dom πp ≡ dom π⌝.
+Proof.
+  iIntros "Hwps".
+  iPoseProof (big_sepM2_dom with "Hwps") as "%Hdomeq".
+  iPureIntro; by rewrite Hdomeq.
+Qed.
+
+(* Isolate a specific thread in a [WPTP]. *)
 Lemma WPTP_extract_wp `{!osirisGS Σ} π πp ι e :
   ⌜π !! ι = Some e⌝ -∗
   WPTP π πp -∗
@@ -81,56 +143,90 @@ Proof.
   by iPureIntro.
 Qed.
 
-Lemma WPTP_extract_posts `{!osirisGS Σ} π πp :
-  WPTP π πp ⊢ ∀ ι o, ⌜π !! ι ≫= is_outcome = Some o⌝ -∗ ∃ γ φ, ⌜πp !! ι = Some (γ, φ)⌝ ∗ (|={⊤}=> □ φ o).
+(* Reinsert a thread that was extracted back into a [WPTP]. *)
+Lemma WPTP_insert_delete `{!osirisGS Σ} ι π1 πp m' γ φ :
+  ⌜πp !! ι = Some (γ, φ)⌝ -∗
+  WPTP (delete ι π1) (delete ι πp) -∗
+  (saved_pred_own γ DfracDiscarded φ ∗ EWP m' <|(ι, ⊥)|> {{ λ o, □ φ o }}) -∗
+  WPTP (<[ι:=m']> π1) πp.
 Proof.
-  iIntros "Hwps" (ι o Hlookup).
-  unfold mbind in Hlookup.
-  apply bind_Some in Hlookup.
-  destruct Hlookup as (m & Hlookup & Houtcome).
-  iPoseProof (big_sepM2_delete_l with "Hwps")
-    as "(%p & %Hlookup_p & H & Hwps)".
-  apply Hlookup. destruct p as [γ φ]. iDestruct "H" as "[? Hwp]".
-  iExists γ, φ.
-  iFrame "%".
-  destruct m; inversion Houtcome.
-  - iApply (ewp_ret_inv with "Hwp").
-  - iApply (ewp_throw_inv with "Hwp").
+  iIntros "%Hlookup Hwps Hwp".
+  replace πp with (<[ι:=(γ, φ)]>πp) by apply (insert_id πp ι (γ, φ) Hlookup).
+  iApply big_sepM2_insert_delete.
+  replace πp with (<[ι:=(γ, φ)]>πp) at 2 by apply (insert_id πp ι (γ, φ) Hlookup).
+  iFrame.
 Qed.
 
+(* Reinsert a terminated thread's postcondition that was extracted
+   back into a [WPTP]. *)
+Lemma WPTP_insert_post_delete `{!osirisGS Σ} ι π1 πp γ φ o :
+  ⌜πp !! ι = Some (γ, φ)⌝ -∗
+  ⌜π1 !! ι = Some (inject2 o)⌝ -∗
+  WPTP (delete ι π1) (delete ι πp) -∗
+  saved_pred_own γ DfracDiscarded φ -∗
+  (|={⊤}=> □ φ o) -∗
+  WPTP π1 πp.
+Proof.
+  iIntros "%Hlookup_p %Hlookup Hwps Hsaved Hwp".
+  replace πp with (<[ι:=(γ, φ)]>πp) by apply (insert_id πp ι (γ, φ) Hlookup_p).
+  replace π1 with (<[ι:=inject2 o]>π1) by apply (insert_id π1 ι (inject2 o) Hlookup).
+  iApply big_sepM2_insert_delete.
+  replace πp with (<[ι:=(γ, φ)]>πp) at 2 by apply (insert_id πp ι (γ, φ) Hlookup_p).
+  replace π1 with (<[ι:=inject2 o]>π1) at 2 by apply (insert_id π1 ι (inject2 o) Hlookup).
+  iFrame.
+  iApply ewp_fupd. iMod "Hwp". iModIntro.
+  iApply ewp_outcome2.
+  iAssumption.
+Qed.
+
+(* Isolate a specific postcondition (i.e. terminated thread) in a [WPTP]. *)
+Lemma WPTP_extract_outcome `{!osirisGS Σ} π πp ι o :
+  ⌜π !! ι = Some (inject2 o)⌝ -∗
+  WPTP π πp -∗
+  ∃ γ φ, ⌜πp !! ι = Some (γ, φ)⌝ ∗ saved_pred_own γ DfracDiscarded φ ∗ WPTP (delete ι π) (delete ι πp) ∗ (|={⊤}=> □ φ o).
+Proof.
+  iIntros "%Hlookup Hwps".
+  iPoseProof (WPTP_extract_wp $! Hlookup with "Hwps") as "(%γ & %φ & %Hlookup_p & #Hsaved & Hwp & Hwps)".
+  iExists γ, φ. iFrame "∗%#".
+  by iApply (ewp_outcome2_inv with "Hwp").
+Qed.
+
+
 Include ewp_rules_tactics.
+
+Ltac invert_can_progress :=
+    lazymatch goal with
+    | h: can_progress _ _ ?e |- _ =>
+        let hstep := fresh "Htstep" in
+        let ι' := fresh "ι'" in
+        let k := fresh "k" in
+        let Heq_e := fresh "Heq_e" in
+        let Hdom := fresh "Hdom" in
+        let v1 := fresh "v" in
+        let v2 := fresh "v" in
+        let u := fresh "u" in
+        let σ'_inner := fresh "σ_inner" in
+        let e'_inner := fresh "e_inner" in
+        let Hstep := fresh "Hstep" in
+        apply invert_can_progress in h as hstep;
+        destruct hstep as
+          [(ι' & k & Heq_e & Hdom)
+          | [ (v1 & v2 & k & Heq_e) |
+              [ (u & k & Heq_e)
+              | ([σ'_inner e'_inner] & Hstep)
+          ] ] ];
+        try subst e
+    end.
+
+Local Ltac iModFL_tac s := iMod s; iModIntro; iNext; iMod s; iModIntro.
+
+Local Tactic Notation "iModFL" constr(s) "as" constr(s') :=
+  iModFL_tac s; iDestruct s as s'.
+Local Tactic Notation "iModFL" constr(s) := iModFL_tac s.
 
 (* Compositional Lemmas for Adequacy *)
 Section satisfiability_weakest_pre.
   Context `{!osirisGS Σ}.
-
-  Lemma ewp_not_stuck {A X} m F E (e : micro A X) ι σ πp Φ n:
-    SAT m F [view E; supply n] (state_interp (σ, πp) ∗ EWP e @ E <| (ι, ⊥) |> {{ Φ }}) →
-    not_stuck e σ (dom πp).
-  Proof.
-    intros Hsat. rewrite /not_stuck.
-    rewrite ewp_unfold /ewp_pre /= in Hsat.
-    ewp_case e; simpl in Hsat.
-    left; by destruct o.
-    all: right.
-    - exfalso.
-      apply SAT_frame_cons in Hsat.
-      apply SAT_fupd in Hsat.
-      by apply SAT_elim in Hsat.
-    - exfalso.
-      apply SAT_frame_cons in Hsat.
-      apply SAT_fupd in Hsat.
-      rewrite /prot upcl_bottom in Hsat.
-      by apply SAT_elim in Hsat.
-    - rewrite Hhm in Hsat.
-      eapply SAT_mono with (Q := (|={E, ∅}=> ⌜can_progress σ (dom πp) e⌝)%I) in Hsat.
-      { eapply SAT_fupd, SAT_elim in Hsat.
-        by left. }
-      iIntros "[Hsi Hwp]".
-      spec_state. iModIntro.
-     by iPureIntro.
-    - right. done.
-  Qed.
 
   Lemma EWP_not_stuck_post {A X} E (e : micro A X) ι σ πp Φ :
     state_interp (σ, πp) ∗ EWP e @ E <| (ι, ⊥) |> {{ Φ }} ={E}[∅]▷=∗
@@ -139,87 +235,59 @@ Section satisfiability_weakest_pre.
     iIntros "(Hsi & Hwp)". rewrite /not_stuck.
     ewp_unfold e.
     ewp_case e; simpl.
-    - ewp_mask_intro "Hmod". iNext. iMod "Hmod". iMod "Hwp". iModIntro.
+    - (* Case: [e] is an [outcome2]. *)
+      ewp_mask_intro "Hmod". iNext. iMod "Hmod". iMod "Hwp". iModIntro.
       iSplitR.
-      + iPureIntro; left; by destruct o.
-      + iIntros (o' Hlookup); unfold inject2 in Hlookup.
-        destruct o; destruct o'; try discriminate Hlookup; inversion Hlookup; iApply "Hwp".
-    - by iMod "Hwp".
-    - rewrite /prot upcl_bottom.
+      + (* Prove we are not stuck. *)
+        iPureIntro; left; by destruct o.
+      + (* Prove we satisfy the postcondition. *)
+        iIntros (o' Heq).
+        destruct o; destruct o'; unfold inject2 in Heq;
+          inversion Heq; iApply "Hwp".
+    - (* Case: [e] is a [crash]. *) by iMod "Hwp".
+    - (* Case: [e] is a [perform]. *)
+      rewrite /prot upcl_bottom.
       by iMod "Hwp".
-    -
+    - (* Case: [e] takes a thread_step. *)
       spec_state. rename Hstep into Hprog.
-      apply invert_can_progress in Hprog as Hstep.
-      destruct Hstep as [Hstep|Hstep].
-      { destruct Hstep as (ι' & k & -> & Hdom).
-        discriminate Hhm. }
-      destruct Hstep as [Hstep|Hstep].
-      { destruct Hstep as (v1 & v2 & k & ->).
-        epose proof (ForkS σ ι (dom πp) v1 v2 k (fresh (dom πp)) (is_fresh _)).
-        Unshelve.
+      invert_can_progress.
+      + (* Subcase: [e] is a join. *)
+        discriminate Hhm.
+      + (* Subcase: [e] is a fork. *)
+        epose proof (ForkS σ ι (dom πp) _ _ k (fresh (dom πp)) (is_fresh _)) as Htstep_fork.
         spec_step.
         iModIntro. iNext. iMod "Hwp". iModIntro.
         iSplitR.
-        + iPureIntro.
-          right; left.
-          apply can_progress_fork.
-        + iIntros (o HFalse). destruct o; discriminate HFalse. }
-      destruct Hstep as [Hstep|Hstep].
-      { destruct Hstep as (u & k & ->).
-        epose proof (SelfS σ (dom πp) ι u k).
+        * (* Prove that we are not stuck. *)
+          iPureIntro. right; left. apply can_progress_fork.
+        * (* Prove that if we are final, we satisfy the post (we are not final). *)
+          iIntros (o HFalse). destruct o; discriminate HFalse.
+      + (* Subcase: [e] is a self. *)
+        epose proof (SelfS σ (dom πp) ι u k) as Htstep_self.
         spec_step.
         iModIntro. iNext. iMod "Hwp". iModIntro.
         iSplitR.
-        + iPureIntro.
-          right; left.
-          apply can_progress_self.
-        + iIntros (o HFalse). destruct o; discriminate HFalse. }
-      destruct Hstep as ([??] & ?).
-      pose proof (BaseS e σ ι m s (dom πp) H).
-      spec_step. iModIntro. iNext. iMod "Hwp". iModIntro.
-      iSplitR.
-      + iPureIntro.
-        right; left.
-        assumption.
-      + iIntros (o HFalse).
-        rewrite HFalse in H0.
-        dependent destruction H0.
-        destruct o; dependent destruction H0.
-        destruct o; discriminate x.
-    - spec_state.
+        * (* Prove that we are not stuck. *)
+          iPureIntro. right; left. apply can_progress_self.
+        * (* Prove that if we are final, we satisfy the post (we are not final). *)
+          iIntros (o HFalse). destruct o; discriminate HFalse.
+      + (* Subcase: [e] takes a regular step. *)
+        pose proof (BaseS e σ ι _ _ (dom πp) Hstep) as Htstep_base.
+        spec_step. iModIntro. iNext. iMod "Hwp". iModIntro.
+        iSplitR.
+        * (* Prove that we are not stuck. *)
+          iPureIntro. right; left. exact Hprog.
+        * (* Prove that if we are final, we satisfy the post (we are not final). *)
+          iIntros (o HFalse); rewrite HFalse in Hstep.
+          destruct o; inversion Hstep.
+    - (* Case: [e] is a join. *)
+      spec_state.
       ewp_mask_intro "Hmod". iNext. iMod "Hmod". iModIntro.
       iSplitR.
-      + iPureIntro.
-        by right; right.
-      + iIntros (o HFalse). destruct o; discriminate HFalse.
-  Qed.
-
-  Lemma ewp_postcondition {A X} m F E Ψ (e : micro A X) (Φ : outcome2 A X -> iProp Σ) v n:
-    SAT m F [view E; supply n] (EWP e @ E <|Ψ|> {{ Φ }}) →
-    outcome2_opt e = Some v →
-    SAT m F [view E; supply n] (Φ v).
-  Proof.
-    intros Hsat Hval. eapply SAT_mono in Hsat; last first.
-    { iIntros "Hwp".
-      destruct e; try discriminate Hval; inversion Hval.
-      - iPoseProof (ewp_ret_inv with "Hwp") as "Hret".
-        rewrite H0. iApply "Hret".
-      - iPoseProof (ewp_throw_inv with "Hwp") as "Hthrow".
-        iApply "Hthrow". }
-    by eapply SAT_fupd in Hsat.
-  Qed.
-
-  Lemma EWP_postcondition {A X} E Ψ (e : micro A X) (Φ : outcome2 A X -> iProp Σ) v :
-    ⌜outcome2_opt e = Some v⌝ -∗
-    (EWP e @ E <|Ψ|> {{ Φ }}) ={E}=∗
-    Φ v.
-  Proof.
-    iIntros "%Hval Hwp".
-    destruct e; try discriminate Hval; inversion Hval.
-    - iPoseProof (ewp_ret_inv with "Hwp") as "Hret".
-      iApply "Hret".
-    - iPoseProof (ewp_throw_inv with "Hwp") as "Hthrow".
-      iApply "Hthrow".
+      + (* Prove that we are not stuck. *)
+        iPureIntro. by right; right.
+      + (* Prove that if we are final, we satisfy the post (we are not final). *)
+        iIntros (o HFalse). destruct o; discriminate HFalse.
   Qed.
 
   Inductive nsteps {A X} : nat → config A X → config A X → Prop :=
@@ -229,36 +297,6 @@ Section satisfiability_weakest_pre.
       step ρ1 ρ2 →
       nsteps n ρ2 ρ3 →
       nsteps (S n) ρ1 ρ3.
-
-  Lemma sat_wp_step {A X} m F E ι Ψ (e1 : micro A X) σ1 πp e2 σ2 μ Φ n :
-    thread_step (σ1, e1, ι, dom πp) (σ2, e2, μ) →
-    SAT m F [view E; supply n]
-      (state_interp (σ1, πp) ∗ EWP e1 @ E <| (ι, Ψ) |> {{ Φ }}) →
-    ∃ n', SAT m F [view E; supply n']
-            (EWP e2 @ E <| (ι, Ψ) |> {{ Φ }} ∗
-            (match μ with
-             | None => state_interp (σ2, πp)
-             | Some (ι', e') =>
-                 ∃ φ' γ, state_interp (σ2, <[ι':=γ]> πp) ∗
-                         saved_prop.saved_pred_own γ DfracDiscarded φ' ∗
-                         EWP e' @ E <| (ι', ⊥) |> {{ λ o : outcome2 val exn, □ φ' o }}
-             end)).
-  Proof.
-    intros Hstep Hsat. eapply SAT_mono in Hsat; last first.
-    { iIntros "[HSI Hwp]". rewrite ewp_unfold /ewp_pre.
-      rewrite (thread_step_is_WPStep _ _ _ _ _ _ _ Hstep).
-      iSpecialize ("Hwp" with "HSI").
-      iExact "Hwp". }
-    eapply SAT_fupd in Hsat.
-    eapply SAT_mono in Hsat; last first.
-    { iIntros "[_ Hwp]". iSpecialize ("Hwp" $! _ _ _ Hstep). iExact "Hwp". }
-    eapply (SAT_frame_resource _ (view ∅)) in Hsat; last apply _.
-    eapply SAT_unframe_resource in Hsat.
-    eapply SAT_fupd in Hsat.
-    eapply SAT_later in Hsat.
-    eapply SAT_fupd in Hsat.
-    eexists n. apply Hsat.
-  Qed.
 
   Lemma ewp_join_inv {A X} γ φ σ πp ι' (k : _ → micro A X) ι Ψ Φ E o :
     ⌜πp !! ι' = Some γ⌝ -∗
@@ -275,308 +313,228 @@ Section satisfiability_weakest_pre.
     ewp_mask_elim. iMod "Hwp" as "($ & $)". done.
   Qed.
 
-  Lemma ewp_self_inv {A X} σ π ι (k : _ -> micro A X) Ψ Φ E :
-    state_interp (σ, π) -∗
-    EWP Stop CSelf () k @ E <|(ι, Ψ)|> {{ Φ }} -∗
-    |={E}[∅]▷=> state_interp (σ, π) ∗ EWP (continue k (VThread ι)) @ E <| (ι, Ψ) |> {{ Φ }}.
-  Proof.
-    iIntros "Hsi Hwp".
-    ewp_unfold (Stop CSelf () k). spec_state.
-    epose proof (SelfS _ _ _ _ _) as Hwpstep.
-    iSpecialize ("Hwp" $! _ _ _ Hwpstep).
-    ewp_mask_elim. iMod "Hwp" as "($ & $)". done.
-  Qed.
-
+  (* Relating a "real" threadpool step (from the definition of the semantics),
+     to a "local" thread step (from the definition of our weakest pre). *)
   Lemma threadpool_thread_step (σ1 σ2 : store) (π1 π2 : thpool) :
+    (* If the threadpool can take a step *)
     threadpool_step (σ1, π1) (σ2, π2) →
+    (* Then either that step was a join *)
     (∃ ι ι' k m,
         π1 !! ι = Some (Stop CJoin ι' k) ∧
         attempt_join ι' π1 k = Some m ∧
         σ1 = σ2 ∧
-        π2 = <[ι:=m]>π1) ∨
+          π2 = <[ι:=m]>π1)
+    ∨
+    (* Or that step can be emulated by a [thread_step]. *)
     ∃ (ι : thread) (m m' : microvx) μ,
       π1 !! ι = Some m ∧
       π2 !! ι = Some m' ∧
       thread_step (σ1, m, ι, dom π1) (σ2, m', μ) ∧
+      (* With different descriptions of [π2] depending on
+         whether a new thread was forked or not. *)
       match μ with
       | None => π2 = <[ι:=m']>π1
       | Some (ι', mf) => <[ι:=m']> π1 !! ι' = None ∧ π2 = <[ι':=mf]>(<[ι:=m']>π1)
       end.
   Proof.
-    inversion 1.
-    - right.
-      eapply BaseS in H5.
+    intros Htpstep.
+    inversion_clear Htpstep.
+    - (* BaseTP case: π !! ι = Some m, step (σ, m) (σ', m') *)
+      right; rename H into Hlookup, H0 into Hstep; subst.
+      eapply BaseS in Hstep as Htstep.
       exists ι, m, m', None.
-      split; first assumption.
-      split; first apply lookup_insert.
-      split; first eassumption.
-      reflexivity.
-    - right.
+      split; [exact Hlookup | split; [apply lookup_insert | split; [exact Htstep | reflexivity]]].
+    - (* ForkTP case: π !! ι = Some (Stop CFork ...), π !! ι' = None *)
+      right; rename H into Hlookup, H0 into Hfresh; subst.
       exists ι, (Stop CFork (v1, v2) k), (continue k (VThread ι')), (Some (ι', call v1 v2)).
-      split; first assumption.
-      split; first (rewrite lookup_insert_ne; first apply lookup_insert).
-      intros ->; rewrite H5 in H3; discriminate.
+      split; [exact Hlookup | ].
+      split; [rewrite lookup_insert_ne; [apply lookup_insert | ] | ].
+      { intros Heq_ι. subst ι'. rewrite Hfresh in Hlookup. discriminate Hlookup. }
       split.
-      + apply ForkS. apply (not_elem_of_dom π1). assumption.
-      + split; last reflexivity.
-        rewrite lookup_insert_ne. assumption.
-        intros ->. rewrite H5 in H3; discriminate.
-    - left. repeat eexists; eassumption.
-    - right.
+      + apply ForkS. apply (not_elem_of_dom π1). exact Hfresh.
+      + split; [| reflexivity].
+        rewrite lookup_insert_ne; [exact Hfresh | ].
+        intros Heq_ι'. subst ι'. rewrite Hfresh in Hlookup. discriminate Hlookup.
+    - (* JoinTP case: π !! ι = Some (Stop CJoin ...), attempt_join ... *)
+      left; rename H into Hlookup, H0 into Hattempt; subst.
+      exists ι, ι', k, m.
+      split; [exact Hlookup | split; [exact Hattempt | split; reflexivity]].
+    - (* SelfTP case: π !! ι = Some (Stop CSelf ...) *)
+      right; rename H into Hlookup; subst.
       exists ι, (Stop CSelf () k), (continue k (VThread ι)), None.
-      split; first assumption.
-      split; first apply lookup_insert.
-      split; last reflexivity.
-      apply SelfS.
-  Qed.
-
-  Lemma WPTP_insert_delete ι π1 πp m' γ φ :
-    ⌜πp !! ι = Some (γ, φ)⌝ -∗
-    WPTP (delete ι π1) (delete ι πp) -∗
-    (saved_pred_own γ DfracDiscarded φ ∗ EWP m' <|(ι, ⊥)|> {{ λ o, □ φ o }}) -∗
-    WPTP (<[ι:=m']> π1) πp.
-  Proof.
-    iIntros "%Hlookup Hwps Hwp".
-    replace πp with (<[ι:=(γ, φ)]>πp) by apply (insert_id πp ι (γ, φ) Hlookup).
-    iApply big_sepM2_insert_delete.
-    replace πp with (<[ι:=(γ, φ)]>πp) at 2 by apply (insert_id πp ι (γ, φ) Hlookup).
-    iFrame.
-  Qed.
-
-  Lemma WPTP_insert_post_delete ι π1 πp γ φ o :
-    ⌜πp !! ι = Some (γ, φ)⌝ -∗
-    ⌜π1 !! ι = Some (inject2 o)⌝ -∗
-    WPTP (delete ι π1) (delete ι πp) -∗
-    saved_pred_own γ DfracDiscarded φ -∗
-    (|={⊤}=> □ φ o) -∗
-    WPTP π1 πp.
-  Proof.
-    iIntros "%Hlookup_p %Hlookup Hwps Hsaved Hwp".
-    replace πp with (<[ι:=(γ, φ)]>πp) by apply (insert_id πp ι (γ, φ) Hlookup_p).
-    replace π1 with (<[ι:=inject2 o]>π1) by apply (insert_id π1 ι (inject2 o) Hlookup).
-    iApply big_sepM2_insert_delete.
-    replace πp with (<[ι:=(γ, φ)]>πp) at 2 by apply (insert_id πp ι (γ, φ) Hlookup_p).
-    replace π1 with (<[ι:=inject2 o]>π1) at 2 by apply (insert_id π1 ι (inject2 o) Hlookup).
-    iFrame.
-    iApply ewp_fupd. iMod "Hwp". iModIntro.
-    iApply ewp_outcome2.
-    iAssumption.
+      split; [exact Hlookup | split; [apply lookup_insert | split; [apply SelfS | reflexivity]]].
   Qed.
 
   Lemma wptp_tstep (π1 : thpool) (πp : gmap thread (gname * (outcome2 val exn → iProp Σ))) σ1 σ2 m m' ι μ :
     ⌜π1 !! ι = Some m⌝ -∗
-    (state_interp (σ1, fst <$> πp) ∗ WPTP π1 πp) -∗
-    ⌜thread_step (σ1, m, ι, dom πp) (σ2, m', μ)⌝ ={⊤}[∅]▷=∗
+    ⌜thread_step (σ1, m, ι, dom πp) (σ2, m', μ)⌝ -∗
+    (state_interp (σ1, fst <$> πp) ∗ WPTP π1 πp) ={⊤}[∅]▷=∗
      match μ with
      | None => state_interp (σ2, fst <$> πp) ∗ WPTP (<[ι:=m']>π1) πp
      | Some (ι', mforked) => ∃ (φ : outcome2 val exn → iProp Σ) γ,
        state_interp (σ2, <[ι':=γ]>(fst <$> πp)) ∗ WPTP (<[ι':=mforked]> (<[ι:=m']>π1)) (<[ι':=(γ, φ)]>πp)
      end.
   Proof.
-    iIntros "%Hlookup [Hsi Hwps] %Hstep".
-    iPoseProof (big_sepM2_dom with "Hwps") as "%Hdomeq".
-    assert (dom πp ≡ dom π1) as Hdomequiv by (rewrite Hdomeq; reflexivity).
+    iIntros "%Hlookup %Hstep [Hsi Hwps]".
+    iPoseProof (WPTP_dom_equiv with "Hwps") as "%Hdomeq".
     iPoseProof (WPTP_extract_wp $! Hlookup with "Hwps")
       as "(%γ & %φ & %Hlookup_p & #Hsaved & Hwp & Hwps)".
-    iPoseProof (ewp_step with "Hsi Hwp") as "Hwp". { rewrite dom_fmap_L. apply Hstep. }
-    iMod "Hwp"; ewp_mask_elim; iMod "Hwp". ewp_mask_elim; iMod "Hwp" as "[Hwp Hrest]".
-    iModIntro.
-    inversion Hstep; subst.
-    - iFrame.
+    iPoseProof (ewp_step with "Hsi Hwp") as ">Hwp". { rewrite dom_fmap_L. apply Hstep. }
+    iModFL "Hwp" as "[Hwp Hμ]".
+    inversion Hstep; subst; iFrame.
+    - (* Case: thread_step is a [BaseS]. *)
       iApply (WPTP_insert_delete $! Hlookup_p with "Hwps [$]").
-    - iDestruct "Hrest" as "(%φ' & %γ' & Hsi & #Hsaved' & Hcall)".
+    - (* Case: thread_step is a [ForkS]. *)
+      iDestruct "Hμ" as "(%φ' & %γ' & Hsi & #Hsaved' & Hcall)".
       iFrame. iExists φ'.
       iPoseProof (WPTP_insert_delete $! Hlookup_p with "Hwps [$]") as "Hwps".
       iApply big_sepM2_insert.
-      rewrite lookup_insert_ne. apply not_elem_of_dom. rewrite Hdomeq. assumption.
-      { intros ->.
-        rewrite (not_elem_of_dom_1 _ _ H0) in Hlookup_p.
-        discriminate Hlookup_p. }
-      apply not_elem_of_dom. assumption.
+      { setoid_rewrite Hdomeq in H0. apply not_elem_of_dom in H0.
+        rewrite lookup_insert_ne; try assumption.
+        apply (lookup_ne π1). by rewrite H0 Hlookup. }
+      { apply not_elem_of_dom; assumption. }
       iFrame. iApply "Hsaved'".
-    - iFrame.
-      iApply (WPTP_insert_delete $! Hlookup_p with "Hwps [Hsaved Hwp]").
-      iFrame. iApply "Hsaved".
+    - (* Case: thread_step is a [SelfS]. *)
+      iApply (WPTP_insert_delete $! Hlookup_p with "Hwps [$ Hwp]").
+      iApply "Hsaved".
   Qed.
 
-  Fixpoint add_posts {A : Type} l (πp : gmap thread A) :=
-    match l with
-    | [] => πp
-    | (ι, φ) :: t => <[ι:=φ]>(add_posts t πp)
+  Ltac invert_threadpool_step :=
+    lazymatch goal with
+    | h: threadpool_step (?σ1, ?π1) (?σ2, ?π2) |- _ =>
+        let Hsteps := fresh "Hsteps" in
+        (have Hsteps := threadpool_thread_step σ1 σ2 π1 π2 h);
+        destruct Hsteps as
+          [ (ι & ι' & k & e & Hlookup & Hattempt & Heq_σ & Heq_π2)
+          | (ι & e & e' & μ & Hlookup & Hlookup' & Htstep & Hμ)
+          ];
+        subst;
+        last first
     end.
 
-  Lemma add_posts_app {A : Type} l l' (πp : gmap thread A) :
-    add_posts (l' ++ l) πp = add_posts l' (add_posts l πp).
-  Proof.
-    induction l' as [ | [ι' φ'] l'].
-    - reflexivity.
-    - simpl. f_equal.
-      apply IHl'.
-  Qed.
-
-  Lemma add_posts_lookup_not_in {A} ι l (πp : gmap thread A) :
-    ι ∉ fst <$> l →
-    add_posts l πp !! ι = πp !! ι.
-  Proof.
-    induction l as [| [ι' a] l IH]; first done.
-    rewrite fmap_cons not_elem_of_cons. simpl.
-    intros [Hneq Hnin].
-    rewrite lookup_insert_ne; first by apply IH.
-    by symmetry.
-  Qed.
-
-  Lemma WPTP_extract_outcome `{!osirisGS Σ} π πp ι o :
-    ⌜π !! ι = Some (inject2 o)⌝ -∗
-    WPTP π πp -∗
-    ∃ γ φ, ⌜πp !! ι = Some (γ, φ)⌝ ∗ saved_pred_own γ DfracDiscarded φ ∗ WPTP (delete ι π) (delete ι πp) ∗ (|={⊤}=> □ φ o).
-  Proof.
-    iIntros "%Hlookup Hwps".
-    iPoseProof (WPTP_extract_wp $! Hlookup with "Hwps") as "(%γ & %φ & %Hlookup_p & #Hsaved & Hwp & Hwps)".
-    iExists γ, φ. iFrame "∗%#".
-    by iApply (ewp_outcome2_inv with "Hwp").
-  Qed.
-
   Lemma wptp_step (π1 π2 : thpool) (πp : gmap thread (gname * (outcome2 val exn → iProp Σ))) σ1 σ2 :
-    (state_interp (σ1, fst <$> πp) ∗ WPTP π1 πp) -∗
-    ⌜threadpool_step (σ1, π1) (σ2, π2)⌝ ={⊤}[∅]▷=∗
+    ⌜threadpool_step (σ1, π1) (σ2, π2)⌝ -∗
+    (state_interp (σ1, fst <$> πp) ∗ WPTP π1 πp) ={⊤}[∅]▷=∗
     (∃ (l : list (thread * (gname * (outcome2 val exn → iProp Σ)))),
         ⌜∀ ι', ι' ∈ fst <$> l → ι' ∉ dom (πp)⌝ ∗
-        state_interp (σ2, fst <$> (add_posts l πp)) ∗ WPTP π2 (add_posts l πp)).
+        state_interp (σ2, fst <$> (insert_list l πp)) ∗ WPTP π2 (insert_list l πp)).
   Proof.
-    iIntros "[Hsi Hwps] %Hstep".
+    iIntros "%Hstep [Hsi Hwps]".
     iPoseProof (WPTP_dom with "Hwps") as "%Hdomeq".
     iCombine "Hsi Hwps" as "Hwps".
-    have Hsteps := threadpool_thread_step σ1 σ2 π1 π2 Hstep.
-    destruct Hsteps; last first.
+    invert_threadpool_step.
     - (* Case: [threadpool_step] is immitated by a [thread_step]. *)
-      destruct H as (ι & e & e' & μ & Hlookup & Hlookup' & Htstep & Hμ).
-      iPoseProof (wptp_tstep $! Hlookup with "Hwps") as "Hwps".
-      rewrite <- Hdomeq in Htstep. iSpecialize ("Hwps" $! Htstep).
-      iMod "Hwps". iModIntro. iNext. iMod "Hwps".
+      rewrite <- Hdomeq in Htstep.
+      iPoseProof (wptp_tstep $! Hlookup Htstep with "Hwps") as "Hwps". (* Use [wptp_tstep]. *)
+      iModFL "Hwps".
       destruct μ as [[ι' mforked] | ]; last first.
       + (* Subcase: the step did not fork any new threads. *)
-        subst π2. iModIntro.
+        subst π2.
         iDestruct "Hwps" as "(Hsi & Hwps)".
         iExists []. iFrame.
         iPureIntro. intros ι' Hin. by apply not_elem_of_nil in Hin.
       + (* Subcase: the step results in a forked thread. *)
-        destruct Hμ as [Hfresh ->].
+        destruct Hμ as [Hfresh Heq_π2]. subst π2.
         iDestruct "Hwps" as "(%φ' & %γ & Hsi & Hwps)".
-        iExists [(ι', (γ, φ'))]. iModIntro.
-        simpl add_posts; rewrite fmap_insert.
+        iExists [(ι', (γ, φ'))].
+        rewrite fmap_insert.
         iFrame.
-        iPureIntro. intros ? Hin. apply elem_of_list_singleton in Hin as ->.
-        simpl. rewrite Hdomeq. apply not_elem_of_dom.
-        assert (ι ≠ ι').
-        { intros ->. rewrite lookup_insert in Hfresh. discriminate Hfresh. }
-        rewrite lookup_insert_ne in Hfresh; last assumption.
-        assumption.
+        iPureIntro. intros ι'' Hin. apply elem_of_list_singleton in Hin as ->.
+        rewrite Hdomeq. apply not_elem_of_dom.
+        assert (ι ≠ ι') as Hneq_ι.
+        { intros Heq_ι. subst ι'. rewrite lookup_insert in Hfresh. discriminate Hfresh. }
+        rewrite lookup_insert_ne in Hfresh; last exact Hneq_ι.
+        exact Hfresh.
     - (* Case: [threadpool_step] is a join. *)
-      destruct H as (ι & ι' & k & e & Hlookup & Hattempt & -> & ->).
       iDestruct "Hwps" as "(Hsi & Hwps)".
       iPoseProof (WPTP_extract_wp $! Hlookup with "Hwps") as "(%γ & %φ & %Hlookup_p & Hsaved & Hwp & Hwps)".
       case (πp !! ι') eqn:Hlookup_p'.
       + (* Case: the join was successful. *)
-        assert (∃ o, π1 !! ι' = Some (inject2 o) ∧ e = k o) as (o & Hlookup' & ->).
+        destruct p as [γ' φ'].
+        assert (∃ o, π1 !! ι' = Some (inject2 o) ∧ e = k o) as (o & Hlookup' & Heq_e).
         { unfold attempt_join in Hattempt.
           assert (is_Some (π1 !! ι')) as [e' Hlookup'].
           { apply elem_of_dom. setoid_rewrite <- Hdomeq.
-            apply (elem_of_dom πp ι'). eexists; eassumption. }
+            apply (elem_of_dom πp ι'). exists (γ', φ'). exact Hlookup_p'. }
           rewrite Hlookup' in Hattempt.
-          destruct e'; inversion Hattempt; try discriminate; rewrite Hlookup'.
-          exists (O2Ret a). split; reflexivity.
-          exists (O2Throw e0). split; reflexivity. }
+          destruct e'; inversion Hattempt; try discriminate; subst; rewrite Hlookup'.
+          - exists (O2Ret a). split; reflexivity.
+          - exists (O2Throw e0). split; reflexivity. }
+        subst e.
         assert (ι ≠ ι') as Hneq.
-        { intros ->. rewrite Hlookup' in Hlookup. inversion Hlookup. destruct o; discriminate. }
-        destruct p as [γ' φ'].
-        assert (delete ι π1 !! ι' = Some (inject2 o)) as Hlookup_del by (rewrite lookup_delete_ne; assumption).
+        { intros Heq_ι. subst ι'. rewrite Hlookup' in Hlookup.
+          inversion Hlookup as [Heq_stop]. destruct o; discriminate Heq_stop. }
+        pose proof (lookup_delete_ne_inv _ _ _ _ Hneq Hlookup') as Hlookup_del.
         iPoseProof (WPTP_extract_outcome (delete ι π1) (delete ι πp) ι' with "[//] Hwps")
           as "(%γ'' & %φ'' & %Hlookup_p'' & #Hsaved' & Hwps & Ho)".
-        assert (delete ι πp !! ι' = Some (γ', φ')) as Hlookup_del_p by (rewrite lookup_delete_ne; [exact Hlookup_p' | done]).
+        pose proof (lookup_delete_ne_inv _ _ _ _ Hneq Hlookup_p') as Hlookup_del_p.
         rewrite Hlookup_del_p in Hlookup_p''. inversion Hlookup_p''; subst γ'' φ''.
         iMod "Ho" as "#Ho".
-        assert ((fst <$> πp) !! ι' = Some γ') as Hlookup_fmap by (rewrite lookup_fmap Hlookup_p'; reflexivity).
+        pose proof (fmap_fst_lookup _ _ _ _ Hlookup_p') as Hlookup_fmap.
         iPoseProof (ewp_join_inv $! Hlookup_fmap with "Hsaved' Ho Hsi Hwp") as "Hwp".
-        iMod "Hwp". iModIntro. iNext. iMod "Hwp". iModIntro.
-        iExists []. simpl. iDestruct "Hwp" as "($ & Hwp)".
-        assert (delete ι π1 !! ι' = Some (inject2 o)) as Hlookup_del' by (rewrite lookup_delete_ne; assumption).
-        iPoseProof (WPTP_insert_post_delete $! Hlookup_del_p Hlookup_del' with "Hwps Hsaved' Ho") as "Hwps".
+        iModFL "Hwp" as "(Hsi & Hwp)".
+        iExists []. iFrame "Hsi".
+        iPoseProof (WPTP_insert_post_delete $! Hlookup_del_p Hlookup_del with "Hwps Hsaved' Ho") as "Hwps".
         iPoseProof (WPTP_insert_delete $! Hlookup_p with "Hwps [$]") as "$".
-        iPureIntro. intros ? Hin. by apply not_elem_of_nil in Hin.
+        iPureIntro. intros ι'' Hin. by apply not_elem_of_nil in Hin.
       + ewp_unfold (Stop CJoin ι' k). spec_state.
         iMod "Hwp".
         assert ((fst <$> πp) !! ι' = None) as Hnin.
-        { apply not_elem_of_dom. rewrite dom_fmap. apply not_elem_of_dom. assumption. }
+        { apply not_elem_of_dom. rewrite dom_fmap. apply not_elem_of_dom. exact Hlookup_p'. }
         setoid_rewrite Hnin.
         by repeat iMod "Hwp".
   Qed.
 
-  Lemma not_elem_of_add_posts {A} ι l (πp : gmap thread A) :
-    ι ∉ dom (add_posts l πp) →
-    ι ∉ fst <$> l ∧ ι ∉ dom πp.
-  Proof.
-    induction l as [| [ι' a] l IH].
-    - simpl.
-      intros Hnin.
-      split; [ apply not_elem_of_nil | assumption ].
-    - simpl. rewrite dom_insert.
-      rewrite not_elem_of_union not_elem_of_singleton.
-      intros [Hnhead Hndom].
-      destruct (IH Hndom) as [Hnlist Hndom'].
-      rewrite not_elem_of_cons.
-      auto.
-  Qed.
-
   Lemma wptp_steps k π1 π2 σ1 σ2 πp :
-    state_interp (σ1, fst <$> πp) ∗ WPTP π1 πp -∗
-    ⌜threadpool_steps k (σ1, π1) (σ2, π2)⌝ ={⊤}[∅]▷=∗^k
+    ⌜threadpool_steps k (σ1, π1) (σ2, π2)⌝ -∗
+    state_interp (σ1, fst <$> πp) ∗ WPTP π1 πp ={⊤}[∅]▷=∗^k
     (∃ (l : list (thread * (gname * (outcome2 val exn → iProp Σ)))),
         ⌜∀ ι', ι' ∈ fst <$> l → ι' ∉ dom (πp)⌝ ∗
-        state_interp (σ2, fst <$> add_posts l πp) ∗ WPTP π2 (add_posts l πp)).
+        state_interp (σ2, fst <$> insert_list l πp) ∗ WPTP π2 (insert_list l πp)).
   Proof.
-    induction k as [|k IH] in  πp, π1, σ1 |-*; iIntros "Hwps %Hsteps".
+    induction k as [|k IH] in  πp, π1, σ1 |-*; iIntros "%Hsteps Hwps".
     - inversion_clear Hsteps. simpl.
       iExists []. iFrame.
       iPureIntro; simpl; intros ? HF.
       by apply not_elem_of_nil in HF.
     - inversion_clear Hsteps as [|?? [σ1' π1']].
       simpl.
-      iPoseProof (wptp_step with "Hwps") as "Hwps".
-      iSpecialize ("Hwps" $! H).
-      iMod "Hwps". iModIntro. iNext. iMod "Hwps" as "(%l & %Hl & Hwps)". iModIntro.
-      iPoseProof (IH with "Hwps") as "Hwps".
-      iSpecialize ("Hwps" $! H0).
+      iPoseProof (wptp_step $! H with "Hwps") as "Hwps".
+      iModFL "Hwps" as "(%l & %Hl & Hwps)".
+      iPoseProof (IH $! H0 with "Hwps") as "Hwps".
       iApply (step_fupdN_wand with "Hwps").
       iIntros "(%l' & %Hl' & Hwps)".
       iExists (l' ++ l).
-      rewrite add_posts_app.
+      rewrite insert_list_app.
       iFrame.
       iPureIntro.
       intros ι' Hin.
       rewrite fmap_app in Hin; apply elem_of_app in Hin.
       destruct Hin.
       + specialize (Hl' ι' H1).
-        apply not_elem_of_add_posts in Hl' as [_ Hndom].
-        assumption.
+        by apply not_elem_of_insert_list in Hl' as [_ Hndom].
       + apply Hl, H1.
   Qed.
 
   (* composing the adequacy lemmas *)
   Lemma wptp_adequacy k σ1 σ2 π2 ι e Φ :
+    ⌜threadpool_steps k (σ1, {[ι:=e]}) (σ2, π2)⌝ -∗
     (∃ γ, state_interp (σ1, {[ι:=γ]}) ∗
           saved_pred_own γ DfracDiscarded (λ o, ⌜Φ o⌝)%I ∗
-          EWP e @ ⊤ <| (ι, ⊥) |> {{ (λ o, □ ⌜Φ o⌝)%I }}) -∗
-    ⌜threadpool_steps k (σ1, {[ι:=e]}) (σ2, π2)⌝ ={⊤}[∅]▷=∗^k
+          EWP e @ ⊤ <| (ι, ⊥) |> {{ (λ o, ⌜Φ o⌝)%I }}) ={⊤}[∅]▷=∗^k
     (∀ ι' e, ⌜π2 !! ι' = Some e⌝ ={⊤}[∅]▷=∗
       ⌜not_stuck e σ2 (dom π2)⌝ ∗
       (∀ o, ⌜π2 !! ι = Some (inject2 o)⌝ -∗ |={⊤}=> □ ⌜Φ o⌝)).
   Proof.
-    iIntros "(%γ & Hsi & Hwps) %Hsteps".
-    rewrite wp_wptp. iCombine "Hsi Hwps" as "Hwps".
+    iIntros "%Hsteps (%γ & Hsi & Hsaved & Hwp)".
+    iPoseProof (ewp_mono with "Hwp []") as "Hwp".
+    { iIntros (o) "%Ho". instantiate (1:=λ o, (□ ⌜Φ o⌝)%I).
+      by iModIntro. }
+    iCombine "Hsi Hsaved Hwp" as "Hwps".
+    rewrite wp_wptp.
     remember {[ι := (γ, λ o, ⌜Φ o⌝)%I]} as πp.
     replace {[ι:=γ]} with (fst <$> πp) by (rewrite Heqπp map_fmap_singleton; reflexivity).
-    iPoseProof (wptp_steps with "Hwps") as "Hwps".
-    iSpecialize ("Hwps" $! Hsteps).
+    iPoseProof (wptp_steps $! Hsteps with "Hwps") as "Hwps".
     iApply (step_fupdN_wand with "Hwps").
     iIntros "(%l & %Hl & Hsi & Hwps)".
     iPoseProof (WPTP_dom with "Hwps") as "%Hdomeq".
@@ -585,23 +543,26 @@ Section satisfiability_weakest_pre.
     iCombine "Hsi Hwp" as "Hwp".
     iPoseProof (EWP_not_stuck_post with "Hwp") as "Hwp".
     rewrite dom_fmap_L Hdomeq.
-    iMod "Hwp". iModIntro. iNext. iMod "Hwp" as "($ & Hpost)".
-    assert (add_posts l πp !! ι = Some (γ, (λ o, ⌜Φ o⌝)%I)) as Hlookup_orig.
-    { rewrite add_posts_lookup_not_in.
+    iModFL "Hwp" as "($ & Hpost)".
+    assert (insert_list l πp !! ι = Some (γ, (λ o, ⌜Φ o⌝)%I)) as Hlookup_orig.
+    { rewrite insert_list_lookup_not_in.
       - by rewrite Heqπp lookup_singleton.
       - intros Hin%Hl. rewrite Heqπp dom_singleton in Hin.
         apply Hin. by apply elem_of_singleton. }
-    case (decide (ι' = ι)) as [-> | Hneq].
-    - iIntros "!>" (o Hlookup').
+    case (decide (ι' = ι)) as [Heq_ι | Hneq].
+    - subst ι'. iIntros (o Hlookup').
       rewrite Hlookup_orig in Hlookup_p.
       rewrite Hlookup' in Hlookup.
-      by inversion Hlookup_p; inversion Hlookup; subst; iApply ("Hpost" $! o eq_refl).
-    - iModIntro. iIntros (o Hlookup_og).
-      assert (delete ι' π2 !! ι = Some (inject2 o)) as Hlookup_del_π2 by (rewrite lookup_delete_ne; assumption).
-      iPoseProof (WPTP_extract_outcome (delete ι' π2) (delete ι' (add_posts l πp)) ι with "[//] Hwps")
+      inversion Hlookup_p; subst γ' φ'.
+      inversion Hlookup; subst e'.
+      by iApply ("Hpost" $! o eq_refl).
+    - iIntros (o Hlookup_og).
+      pose proof (lookup_delete_ne_inv _ _ _ _ Hneq Hlookup_og) as Hlookup_del_π2.
+      iPoseProof (WPTP_extract_outcome (delete ι' π2) (delete ι' (insert_list l πp)) ι with "[//] Hwps")
         as "(%γ'' & %φ'' & %Hlookup_p' & _ & _ & HΦ)".
-      rewrite lookup_delete_ne in Hlookup_p'; last done.
-      by rewrite Hlookup_orig in Hlookup_p'; inversion Hlookup_p'; subst.
+      rewrite lookup_delete_ne in Hlookup_p'; last exact Hneq.
+      rewrite Hlookup_orig in Hlookup_p'. inversion Hlookup_p'; subst γ'' φ''.
+      done.
   Qed.
 
   Lemma ewp_adequacy m F n ι e σ1 σ2 π2 k Φ :
@@ -617,39 +578,28 @@ Section satisfiability_weakest_pre.
     (∀ o, π2 !! ι = Some (inject2 o) → Φ o).
   Proof.
     intros Hsat Hsteps.
-    eapply SAT_mono with
-      (Q:=(∃ γ : gname, state_interp (σ1, {[ι := γ]}) ∗
-                          saved_pred_own γ DfracDiscarded (λ o : outcome2 val exn, ⌜Φ o⌝) ∗
-                          EWP e <|(ι, ⊥)|> {{ λ o : outcome2 val exn, □ ⌜Φ o⌝ }})%I) in Hsat; last first.
-    { iIntros "(%γ & Hsi & Hsaved & Hwp)".
-      iExists γ. iFrame "Hsi Hsaved".
-      iApply (ewp_mono with "Hwp").
-      iIntros (o HΦ). iFrame "%". }
-    eapply SAT_mono in Hsat; last first.
-    iIntros "Hwps".
-    iPoseProof (wptp_adequacy k σ1 σ2 π2 with "Hwps") as "Hx".
-    iSpecialize ("Hx" $! Hsteps). iExact "Hx".
+    eapply SAT_mono in Hsat; last iApply (wptp_adequacy k σ1 σ2 π2 $! Hsteps).
     apply SAT_elim_iterated in Hsat; last first.
-    { intros P HsatP.
-      by apply SAT_fupd, SAT_later, SAT_fupd in HsatP. }
+    { intros P HsatP; by eapply SAT_fupd, SAT_later, SAT_fupd. }
     split.
-    - intros ι' e' Hlookup.
-      eapply SAT_mono in Hsat; last first.
+    - (* Prove that no thread is stuck. *)
+      intros ι' e' Hlookup.
+      eapply SAT_mono in Hsat; last first. (* Instantiate inside SAT. *)
       { iIntros "Hx". iSpecialize ("Hx" $! ι' e' Hlookup). iExact "Hx". }
       apply SAT_fupd, SAT_later, SAT_fupd in Hsat.
-      eapply SAT_mono in Hsat; last first.
+      eapply SAT_mono in Hsat; last first. (* Symmetry inside SAT. *)
       { iIntros "[Hns Ho]". iCombine "Ho Hns" as "Hx". iExact "Hx". }
       rewrite -SAT_frame_cons in Hsat.
-      apply SAT_elim in Hsat.
-      by apply Hsat.
-    - intros o Hlookup.
-      eapply SAT_mono in Hsat; last first.
+      by apply SAT_elim in Hsat.
+    - (* Prove that if the initial thread has terminated,
+         then the postcondition holds. *)
+      intros o Hlookup.
+      eapply SAT_mono in Hsat; last first. (* Instantiate inside SAT. *)
       { iIntros "Hx". iSpecialize ("Hx" $! ι (inject2 o) Hlookup). iExact "Hx". }
       apply SAT_fupd, SAT_later, SAT_fupd in Hsat.
       rewrite -SAT_frame_cons in Hsat.
       eapply SAT_mono in Hsat; last first.
-      { iIntros "HΦ".
-        iSpecialize ("HΦ" $! o Hlookup). iExact "HΦ". }
+      { iIntros "HΦ". iSpecialize ("HΦ" $! o Hlookup). iExact "HΦ". }
       apply SAT_fupd, SAT_pers in Hsat.
       apply SAT_elim in Hsat.
       by apply Hsat.
@@ -724,7 +674,7 @@ Section adequacy.
   (* ------------------------------------------------------------------------ *)
   (** Adequacy Theorem for [EWP] for computations under open gFunctors [Σ]. *)
 
-  Definition osiris_adequacy Σ `{!osirisGpreS Σ} (e : micro val exn) ι σ1 π2 σ2 k Φ :
+  Lemma osiris_adequacy Σ `{!osirisGpreS Σ} (e : micro val exn) ι σ1 π2 σ2 k Φ :
     (* If we can show [EWP e1 {{ True }}] with the ghost state provided by [Σ]. *)
     (∀ `{!osirisGS Σ}, ⊢ EWP e @ ⊤ <|(ι, ⊥)|> {{ λ o, ⌜Φ o⌝ }}) →
     (* then any k-step execution is safe: *)
